fixed tactics, cleaned up f2p proofs

translation/MapUtils.v
@@ -20,52 +20,24 @@ Open Scope list.
 Require Import Stdlib.FSets.FMapInterface.
 Require Import Stdlib.ZArith.ZArith.
 
-Require coqutil.Map.SortedListString.
-Local Existing Instance SortedListString.map.
-Local Existing Instance SortedListString.ok.
-Local Existing Instance SortedListString.Build_parameters.
-
-Require Import Stdlib.Sorting.Permutation.
-
 Require Import Tactics Translator.
+Export Stdlib.Sorting.Permutation.
 
-Ltac invert_cons := repeat (
-  try match goal with
-  | [H: NoDup (?b::?c) |-_] => inversion H; clear H
-  | [H: StronglySorted ?a (?b::?c) |-_] => inversion H; clear H
-  | [H: Permutation [] (?a::?b) |-_] => eapply Permutation_nil in H
-  | [H: Permutation (?a::?b) [] |-_] => eapply Permutation_sym in H; eapply Permutation_nil in H
-  | [H: Permutation ?a ?a |-_] => clear H
-  | [H: Forall2 ?p [] (?a::?b) |-_] => inversion H
-  | [H: Forall2 ?p (?a::?b) [] |-_] => inversion H
-  | [H: Forall ?p (?a::?b) |-_] => eapply Forall_cons
-  end; inj_all).
+Section WithMap.
+  Context {locals: forall T, map.map string T} 
+  {locals_ok: forall T, map.ok (locals T)}.
 
-Hint Constructors Permutation: permute.
-Hint Resolve Permuted_record_sort
-  Permutation_map
-  Permutation_in
-  Permutation_NoDup
-  Permutation_refl
-  Permutation_sym
-  Permutation.Permutation_cons_inv 
-  Permutation_trans: permute.
-Hint Resolve in_eq in_map: core.
-
-
-Definition fenv_wf (Genv: list(string*type)) (fenv:map.rep) :=
+Definition fenv_wf (Genv: list (string*type)) (fenv:tenv) :=
   (Success fenv = fiat_env_to_map Genv) /\
   tenv_wf fenv.
 Hint Unfold fenv_wf: core.
 
-Opaque map.put map.get map.empty.
-
-Theorem fiat_env_to_map_contains {x}{t}{Genv}{fenv:map.rep}:
+Theorem fiat_env_to_map_contains {x}{t}{Genv}{fenv:tenv}:
   Success fenv = fiat_env_to_map ((x,t)::Genv) ->
   tenv_wf fenv -> map.get fenv x = Some t.
 Proof. 
   simpl; intros; repeat (case_match; try discriminate).
-  inversion H; map_simpl.
+  inj_all; map_simpl.
 Qed.
 
 Theorem string_eq_destruct (x:string) (x':string):
@@ -76,7 +48,8 @@ Proof.
   destruct (x=?x'); eauto.
 Qed.
 
-Theorem fiat_env_to_map_contents {x}{t}{Genv}{G}{G'}:
+Theorem fiat_env_to_map_contents:
+  forall x t Genv G G',
   Success G = fiat_env_to_map ((x,t)::Genv) ->
   Success G' = fiat_env_to_map (Genv) ->
   tenv_wf G -> 
@@ -84,10 +57,11 @@ Theorem fiat_env_to_map_contents {x}{t}{Genv}{G}{G'}:
   (x=x' /\ t=t') \/ (map.get G' x' = Some t').
 Proof.
   simpl; intros; inj_all.
-  destruct (string_eq_destruct x' x); repeat (inj_all; map_simpl).
+  destruct (string_eq_destruct x' x); inj_all; map_simpl.
 Qed.
 
-Theorem tenv_wf_ext {fenv:map.rep} {t:type} {s:string}:
+Theorem tenv_wf_ext:
+  forall (fenv:tenv) (t:type) (s:string),
   map.get fenv s = None ->
   tenv_wf (map.put fenv s t) -> tenv_wf fenv.
 Proof.
@@ -97,7 +71,8 @@ Proof.
 Qed.
 Hint Resolve tenv_wf_ext: core.
 
-Theorem fenv_wf_ext {G} {fenv:map.rep} {t:type} {s:string}:
+Theorem fenv_wf_ext:
+  forall (G:list (string*type)) (fenv:tenv) (s:string) (t:type),
   fenv_wf ((s,t)::G) fenv -> 
   type_wf t /\ 
   exists fenv',
@@ -105,7 +80,7 @@ Theorem fenv_wf_ext {G} {fenv:map.rep} {t:type} {s:string}:
   fenv_wf G fenv' /\
   None = map.get fenv' s.
 Proof.
-  intros. destruct H; inj_all; eauto.
+  intros. destruct H; do_both; eauto.
   apply conj.
   - apply H0 with s; map_simpl.
   - eexists; repeat (apply conj); eauto.
@@ -119,23 +94,18 @@ Ltac fenv_reduce := inj_all;
           end); map_simpl; inj_all.
 
 Theorem lookup_fmap:
-  forall Genv {fenv:map.rep} (HFenv: fenv_wf Genv fenv) x t {d},
+  forall Genv {fenv:tenv} (HFenv: fenv_wf Genv fenv) x t {d},
   (exists a, Success a = lookup_ind x Genv /\ t = snd (nth a Genv d))
   <->
   (map.get fenv x = Some t).
 Proof.
   induction Genv;
-  intros. { unfold fenv_wf in HFenv; apply conj; intros; inj_all. }
-  apply conj; intros; fenv_reduce; map_simpl.
-  - eapply IHGenv; eauto.
-  - exists 0; inj_all.
-  - edestruct IHGenv; eauto; clear IHGenv.
-    edestruct H4; eauto; clear H4.
-    inj_all; equality.
-  - edestruct IHGenv; eauto; clear IHGenv.
-    edestruct H4; eauto; clear H4.
-    inj_all; equality.
-  Unshelve. exact ("",TUnit).
+  intros. { unfold fenv_wf in HFenv; apply conj; intros; inj_all; map_simpl. }
+  apply conj; intros; fenv_reduce; do_both; map_simpl.
+  { eapply IHGenv; eauto. }
+  all: edestruct IHGenv; eauto; clear IHGenv;
+    edestruct H4; eauto; clear H4; do_both.
+  Unshelve. all: eauto.
 Qed.
 
 Hint Rewrite lookup_fmap: core. 
@@ -162,15 +132,16 @@ Proof.
 
     invert_cons.
     destruct Hinl' as [Hs'|Hinl']; destruct Hinl as [Hs|Hinl]; invert_cons; try solve [
+      equality;
       apply Permutation.Permutation_cons_inv in H;
       f_equal; eauto
     ].
     pose proof (Forall_In H7 Hinl');
     pose proof (Forall_In H10 Hinl); inj_all.
     unfold is_true, Value.record_entry_leb in *;
-    inj_all.
-    apply String.leb_antisym in H0, H1; inj_all; eauto.
-    assert (In (fst (s,t0)) (map fst l')) by eauto; inj_all.
+    equality.
+    apply String.leb_antisym in H0, H1; do_both; eauto.
+    assert (In (fst (s,t0)) (map fst l')) by eauto; do_both.
 Qed.
 Hint Resolve sorted_perm_eq: core.
 
@@ -198,14 +169,14 @@ Proof.
   unfold record_entry_leb.
   induction a; destruct b; intros; apply conj; intros; invert_cons.
   - apply SSorted_nil.
-  - constructor; try apply IHa; inj_all.
+  - constructor; try apply IHa; equality.
   assert (Hforall: Forall (fun p => (fun q => is_true (s <=? q)) (fst p)) a0) by eauto.
   apply Forall_map_fst in Hforall.
   replace (map fst a0) with (map fst b) in Hforall.
   rewrite <- Forall_map_fst in Hforall.
   eauto.
 Qed.
-Hint Resolve fst_equal_equiv.
+Hint Resolve fst_equal_equiv: core.
 
 Ltac invert_lhs :=
   match goal with [|-?a=_] => set (b:=a); assert (a=b) by eauto; destruct b end.
@@ -215,11 +186,10 @@ Ltac invert_rhs :=
   | [|- _ = ?a] => set (b:=a); assert (a=b) by eauto; destruct b
   | [|- exists _, _ = ?a] => set (b:=a); assert (a=b) by eauto; destruct b end.
 
-
 Definition d:=("",TUnit).
 
 Theorem lookup_fmap_none:
-  forall Genv {fenv:map.rep} (HFenv: fenv_wf Genv fenv) x,
+  forall Genv {fenv:tenv} (HFenv: fenv_wf Genv fenv) x,
   (forall msg, Failure msg = lookup_ind x Genv ->
   map.get fenv x = None) /\
   (map.get fenv x = None ->
@@ -233,22 +203,28 @@ Proof.
     specialize H1 with x (snd (nth a Genv d)) d; inj_all.
     destruct H1.
     lapply H1; eauto.
-    intros; equality.
+    intros; do_both.
 Unshelve. all: eauto.
 Qed.
 Hint Rewrite lookup_fmap_none: core.
 
+Theorem fenv_wf_nil:
+  fenv_wf [] map.empty.
+Proof.
+  unfold fenv_wf, tenv_wf in *; apply conj; intros; map_simpl; inj_all.
+Qed.
+
 Theorem fenv_wf_cons:
-  forall {Genv} {fenv} (HFenv: fenv_wf Genv fenv) 
+  forall {Genv:list(string*type)} {fenv:tenv} (HFenv: fenv_wf Genv fenv) 
   x a {Hnew: map.get fenv x = None} {Htwf: type_wf a},
   fenv_wf ((x,a)::Genv) (map.put fenv x a).
 Proof.
   intros.
-  unfold fenv_wf in *; inj_all.
+  unfold fenv_wf in *; do_both.
   apply conj; eauto. unfold tenv_wf in *; intros; map_simpl; eauto.
   destruct (string_eq_destruct x x0); repeat (inj_all; map_simpl); eauto.
 Qed.
-Hint Resolve fenv_wf_cons: core.
+Hint Resolve fenv_wf_nil fenv_wf_cons: core.
 Hint Resolve StronglySorted_record_sort: core.
 
 Hint Constructors StronglySorted: core.
@@ -262,7 +238,7 @@ Theorem all_success_permutation:
   Permutation.Permutation sl sl'.
 Proof.
   do 4 intro.
-  induction Hp; intros; invert_cons; eauto with permute.
+  induction Hp; intros; invert_cons; do_both; eauto with permute.
 Qed.
 
 Theorem Permutation_forall:
@@ -306,16 +282,5 @@ Qed.
 
 Hint Resolve Forall2_map_left Forall2_map_right Forall2_split: core.
 
-Ltac gather n :=
-  repeat match goal with
-         | [H: n = ?m|-_] => rewrite <- H in *
-         | [H: ?m = n|-_] => rewrite H in *
-         end.
 
-
-Theorem fenv_wf_nil:
-  fenv_wf [] map.empty.
-Proof.
-  unfold fenv_wf in *; apply conj; inj_all.
-Qed.
-Hint Resolve fenv_wf_nil: core.
+End WithMap.
