translation/PyroToFiatSound.v
@@ -4,7 +4,7 @@ From fiat2 Require Import Language TypeSystem TypeSound Value.
 Require Import coqutil.Map.Interface coqutil.Datatypes.dlist.
 From Utils Require Import Utils.
 
-From Pyrosome Require Import Theory.Core Elab.Elab Tools.Matches Lang.SimpleVSubst Tools.EGraph.Automation Tools.EGraph.Defs Tools.UnElab.
+From Pyrosome Require Import Theory.WfCutElim Theory.Core Elab.Elab Tools.Matches Lang.SimpleVSubst Lang.SimpleVSTLC.
 From Pyrosome Require Import Lang.FiatTest.
 Import Core.Notations.
 Import coqutil.Datatypes.Result Result.List Result.ResultMonadNotations.
@@ -19,71 +19,186 @@ Open Scope list.
 
 Require Import Stdlib.FSets.FMapInterface.
 Require Import Stdlib.ZArith.ZArith.
+From Stdlib Require Import Psatz.
 
 Require coqutil.Map.SortedListString.
-Local Existing Instance SortedListString.map.
-Local Existing Instance SortedListString.ok.
-Local Existing Instance SortedListString.Build_parameters.
-
 Require Import Translator MapUtils Tactics.
+Import SimpleVSubst.
 
-Opaque map.put map.get map.empty.
+Section WithMap.
+  Context {locals: forall T, map.map string T} 
+{locals_ok: forall T, map.ok (locals T)}.
 
+  Print wf_args.
+  Notation wf_args l :=
+    (wf_args (Model:= core_model l)).
+
+Definition pyro_wf_fiat_ty (e:term) (t:sort) :=
+  (t = (scon "ty" []) ->
+  forall ft, Success ft = ty_pyro_to_fiat e ->
+  type_wf ft) /\
+  (t = (scon "list_ty" []) -> 
+  forall tl, Success tl = list_ty_pyro_to_fiat e ->
+  Forall type_wf (map snd tl)).
+
+Hint Constructors type_wf: core.
+Hint Resolve conj: core.
+Hint Resolve eq_sort_refl: core.
+
+Search wf_sort.
+Lemma ty_sort_wf: wf_sort fiat_rules [] (scon "ty" []).
+Proof. eapply wf_sort_by; t''; t'. Qed.
+Lemma list_ty_sort_wf: wf_sort fiat_rules [] (scon "list_ty" []).
+Proof. eapply wf_sort_by; t''; t'. Qed.
+Hint Resolve ty_sort_wf list_ty_sort_wf: core.
+
+Check wf_term_cut_ind.
+Opaque fiat_rules.
+
+Lemma ty_sort_eq:
+  forall t c (Heq: eq_sort fiat_rules c t {{s #"ty"}}), 
+  t = {{s #"ty"}}.
+Proof.
+  enough (forall t t' c (Heq: eq_sort fiat_rules c t t'), 
+  t = {{s #"ty"}} <-> t' = {{s #"ty"}}) by (intros; eapply H; eauto).
+
+  intros t t' c Heq.
+  induction Heq; eauto; try easy.
+  - repeat (destruct H; equality).
+  - destruct t1', t2'.
+    induction l; induction l0; compute in *; apply conj; intros; inj_all.
+  - intuition.
+Qed.
+
+Definition pyro_ty_destruct (e:term) (t:sort) :=
+  (t = {{s #"ty"}} ->
+  e = {{e #"nat"}} \/
+  e = {{e #"bool"}} \/
+  e = {{e #"comparison"}} \/
+  (exists l, e = {{e #"list" {l} }} /\ wf_term fiat_rules [] l {{s #"ty"}}) \/
+  (exists l, e = {{e #"Trecord" {l} }} /\ wf_term fiat_rules [] l {{s #"list_ty"}})).
+
+Lemma ty_sort_destruct:
+  forall e t,
+  wf_term fiat_rules [] e t ->
+  pyro_ty_destruct e t.
+Proof.
+  apply wf_term_cut_ind; intros;
+  unfold pyro_ty_destruct in *; inj_all.
+  + intros. repeat (destruct H; equality).
+    all: repeat (destruct s; inj_all).
+    - inversion H0; inj_all.
+      repeat right; eexists; eauto.
+    - inversion H0; inj_all.
+      do 3 right; left. eexists; eauto.
+  + intros. inj_all. eapply ty_sort_eq in H1; inj_all.
+Qed.
+
+Lemma list_ty_sort_eq:
+  forall t c (Heq: eq_sort fiat_rules c t {{s #"list_ty"}}),
+  t = {{s #"list_ty"}}.
+Proof.
+  enough (forall t t' c (Heq: eq_sort fiat_rules c t t'), 
+  t = scon "list_ty" [] <-> t' = scon "list_ty" []) by (intros; eapply H; eauto).
+  intros t t' c Heq.
+  induction Heq; eauto; try easy.
+  - repeat (destruct H; equality).
+  - destruct t1', t2'.
+    induction l; induction l0; compute in *; apply conj; intros; inj_all.
+  - intuition.
+Qed.
+
+Hint Resolve ty_sort_eq list_ty_sort_eq: core.
 
 Theorem ty_pyro_to_fiat_wf:
-  forall (Gp:term) ft,
-  Success ft = ty_pyro_to_fiat Gp ->
-  type_wf ft.
+  forall (Gp:term) (t:sort)
+  (Hpwf: wf_term fiat_rules [] Gp t),
+  (pyro_wf_fiat_ty Gp t).
 Proof.
-  induction ft using type_IH; intros; case_match' Gp; inj_all; 
-  try solve [econstructor].
-Qed.
+  unfold pyro_wf_fiat_ty.
+  apply wf_term_cut_ind; intros; cycle 1.
+  - inj_all.
+  - apply conj; intros; inj_all; eauto.
+  - apply conj; intros.
+    * repeat (destruct H; equality).
+      all: inj_all.
+        enough (type_wf (TRecord a) /\ Forall (fun p => forall q, of_nat q = fst p -> length a > q) a) by intuition.
+        clear H H0 H1.
+        generalize dependent t.
+        induction a; intros; destruct t; try solve [repeat constructor; eauto]; invert_cons.
+        specialize IHa with t0; inj_all.
+        inversion H; inj_all.
+        pose proof Forall_map_fst as Hfst.
+        specialize Hfst with (P:=(fun x => forall q, of_nat q = x -> length a1 > q)); simpl in Hfst.
+        apply Hfst in H0.
+
+        apply conj; constructor; invert_cons; try constructor; eauto.
+        + unfold "~"; intros.
+          From Stdlib Require Import Psatz.
+          eapply Forall_In in H2; try eapply H0; inj_all.
+          specialize H2 with (length a1); inj_all; lia.
+        + admit.
+        + apply of_nat_inj in H2; inj_all.
+          admit.
+        + apply Hfst in H0.
+          eapply Forall_impl; try eapply H0; eauto.
+    * inj_all;
+      repeat (destruct H; equality); inj_all.
+Admitted.
+
 Hint Resolve ty_pyro_to_fiat_wf: core.
-(* just bools for now lol *)
 
-Require Import Psatz.
+Lemma env_sort_eq:
+  forall t c (Heq: eq_sort fiat_rules c t (scon "env" [])), 
+  t = scon "env" [].
+Proof.
+  enough (forall t t' c (Heq: eq_sort fiat_rules c t t'), 
+  t = scon "env" [] <-> t' = scon "env" []) by (intros; eapply H; eauto).
+  intros t t' c Heq.
+  induction Heq; eauto; try easy.
+  - repeat (destruct H; equality).
+  - destruct t1', t2'.
+    induction l; induction l0; compute in *; apply conj; intros; inj_all.
+  - intuition.
+Qed.
+Hint Resolve env_sort_eq: core.
 
-Theorem env_pyro_to_fiat_unique:
-  forall (Genv: list(string*type)) (Gp:term),
-  Success Genv = env_pyro_to_fiat Gp ->
-  exists fenv, 
-  (fenv_wf Genv fenv /\
+Definition env_pyro_to_fiat_wf_term  (Gp:term) (t:sort)  :=
+  forall (Genv: list(string*type))
+  (Hs: t = scon "env" [])
+  (Henv: Success Genv = env_pyro_to_fiat Gp),
+  exists fenv, (fenv_wf Genv fenv /\
   forall t n, map.get fenv (of_nat n) = Some t ->
   n < length Genv).
-Proof.
-  induction Genv; intros; inj_all.
-  - pose fenv_wf_nil; repeat (eexists); inj_all.
-  - case_match' Gp; inj_all.
-    specialize (IHGenv t1); inj_all.
-    eapply fenv_wf_cons with (x:=of_nat (length a0)) in H as Hwf; eauto.
-    * repeat eexists; try eapply Hwf.
-      intros.
-      assert (Hneq: n=length a0 \/ n<>length a0) by lia.
-      destruct Hneq; inj_all; map_simpl.
-      assert (of_nat (length a0) <> of_nat n). {
-        unfold "<>"; intros.
-        apply of_nat_inj in H3. lia.
-        }
-      map_simpl. eapply H0 in H1; lia.
-    * invert_lhs; eauto.
-      apply H0 in H1; lia.
-Qed.
 
 Theorem env_pyro_to_fiat_wf:
-  forall (Genv: list(string*type)) (Gp:term),
-  Success Genv = env_pyro_to_fiat Gp ->
-  exists {fenv:map.rep}, fenv_wf Genv fenv.
+  forall (Gp:term) (t:sort)
+  (Hpwf: wf_term fiat_rules [] Gp t),
+  env_pyro_to_fiat_wf_term Gp t.
 Proof.
-  intros; eauto.
-  pose (env_pyro_to_fiat_unique) as Henv.
-  specialize (Henv Genv Gp H).
-  inj_all; eauto.
+  apply wf_term_cut_ind;
+  unfold env_pyro_to_fiat_wf_term;
+  intros; intuition; inj_all; eauto.
+  - eexists; apply conj; try eapply fenv_wf_nil; intros; map_simpl.
+  - repeat (destruct H; equality).
+    clear H2; specialize H3 with a0; inj_all.
+    eexists; apply conj; try eapply fenv_wf_cons; intros; eauto; map_simpl.
+      * specialize H2 with (n:=length a0). 
+        destruct (map.get x (of_nat (length a0))); inj_all.
+        specialize H2 with t; inj_all. lia.
+      * eapply ty_pyro_to_fiat_wf in case_match_eqn; eauto.
+        inversion H0; eauto.
+      * assert (Hneq: n=length a0 \/ n<>length a0) by lia.
+        destruct Hneq; inj_all. 
+        assert (of_nat (length a0) <> of_nat n). {
+        unfold "<>"; intros. 
+        apply of_nat_inj in H5. lia.
+        }
+        map_simpl. apply H2 in H3; lia.
 Qed.
 
-Compute wf_judge_ind.
+Hint Resolve env_pyro_to_fiat_wf: core.
 
-
-Print wf_term.
 
 (*
    induction on judgement structure...
@@ -96,59 +211,102 @@ Print wf_term.
    desire some kind of alpha-equivalence on the fiat2 side
    define a relation of fiat2 programs "renamable"
    free vs bound variables
+ *) 
+
+Definition pyro_expr_wf (e:term) (t:sort) :=
+  forall A Gp, 
+  t = scon "val" [A;Gp] ->
+  forall fe, Success fe = expr_pyro_to_fiat e ->
+  forall ft Genv fenv,
+  Success ft = ty_pyro_to_fiat A ->
+  Success Genv = env_pyro_to_fiat Gp ->
+  fenv_wf Genv fenv ->
+  type_of map.empty fenv fe ft.
+
+Lemma val_sort_eq:
+  forall t A Gp (Heq: eq_sort fiat_rules [] t (scon "val" [A;Gp]))
+  (Ha: wf_term fiat_rules [] A (scon "ty" []))
+  (HG: wf_term fiat_rules [] Gp (scon "env" [])),
+  exists A' Gp',
+  t = scon "val" [A';Gp'] /\
+  eq_term fiat_rules [] (scon "ty" []) A A' /\ 
+  eq_term fiat_rules [] (scon "env" []) Gp Gp'.
+Proof.
+  intros. 
+  induction Heq; intros; inj_all; eauto.
+  - repeat (destruct H; equality).
+  - induction s1; destruct s2; inversion H; invert_cons.
+    + rewrite sort_subst_nil. 
+      repeat eexists. ; try rewrite term_subst_nil; auto.
+    + clear IHHeq.
+      Search term_subst.
+      inversion Ha; inj_all.
+Unset Printing Notations.
+    Search apply_subst.
+    
+
+
+(*
+Lemma val_sort_eq:
+  forall t c A Gp (Heq: eq_sort fiat_rules c t (scon "val" [A;Gp]))
+  (Ha: wf_term fiat_rules c A (scon "ty" []))
+  (HG: wf_term fiat_rules c Gp (scon "env" [])),
+  t = scon "val" [A;Gp].
+Proof.
+  intros.
+  inj_all.
+  pose proof ty_sort_eq.
+
+
+  enough (forall t t' c (Heq: eq_sort fiat_rules c t t') A Gp,
+  (*(Ha: wf_term fiat_rules c A (scon "ty" []))
+     (HG: wf_term fiat_rules c Gp (scon "env" [])),*)
+  t = scon "val" [A;Gp] <-> t' = scon "val" [A;Gp]) by (intros; eapply H; eauto).
+  intros t t' c Heq.
+  induction Heq; intros; eauto.
+  - intros; subst.
+    repeat (destruct H; equality).
+  - intros; subst.
+    destruct t1', t2'. 
+    apply conj; intros; inversion H1; inj_all.
+    + do 3 (destruct l; inj_all).
+      inversion H4; inj_all.
+      specialize IHHeq with t t0; destruct IHHeq; inj_all.
+      inversion H1; inj_all.
+      enough (term_subst s2 t0 = term_subst s1 t0 /\ term_subst s2 t = term_subst s1 t). {
+        inj_all; f_equal; f_equal; eauto; f_equal; eauto.
+      }
+      f_equal; cbn.
+      
+      Search eq_subst.
+      repeat f_equal.
+
+Qed.
  *)
 
-  Print wf_args.
-  Notation wf_args l :=
-    (wf_args (Model:= core_model l)).
-
-  Locate sort.
-Definition pyro_is_wf_fiat (e:term) (t:SimpleVSubst.sort) :=
-  forall fe, Success fe = expr_pyro_to_fiat e ->
-  exists A Gp ft Genv fenv Gstore fstore,
-  t = scon "val" [A;Gp] /\
-  Success ft = ty_pyro_to_fiat A /\
-  Success Genv = env_pyro_to_fiat Gp /\
-  fenv_wf Gstore fstore /\
-  fenv_wf Genv fenv /\
-  type_of fstore fenv fe ft.
-
-
 Theorem expr_pyro_to_fiat_wf: 
-  (forall c t, wf_sort fiat_rules c t -> True)
-  /\ (forall c e t, wf_term fiat_rules c e t -> pyro_is_wf_fiat e t)
-      /\ (forall c s c', wf_args fiat_rules c s c' -> 
-      Forall2 pyro_is_wf_fiat s (map snd c')).
+  forall (pt:term) (t:sort)
+  (Hpwf: wf_term fiat_rules [] pt t),
+  (pyro_expr_wf pt t).
 Proof.
-  unfold pyro_is_wf_fiat.
-  apply wf_judge_ind; inj_all.
-- intros; repeat (destruct c'; invert_cons); eauto.
-  + basic_goal_prep;
-      basic_core_crush.
-      Search "lookup".
-      Search In.
+  apply wf_term_cut_ind;
+  unfold pyro_expr_wf;
+  intros; intuition.
+  - repeat (destruct H; equality).
+    all: inj_all.
+    all: cbn in *.
+    all: inversion H2; inj_all.
+    all: try solve [repeat econstructor; eauto].
+    + specialize H1 with (con "list" [t1]) Gp a0 (TList a1) Genv fenv; inj_all.
+      repeat econstructor; eauto.
+    + inversion H0; clear H0; inj_all.
+      repeat econstructor; eapply ty_pyro_to_fiat_wf; eauto.
+  - inj_all.
+    inversion H1; inj_all.
+    + repeat (destruct H2; equality).
+    + 
+    
+Qed.
 
 
-Functional Scheme expr_pyro_to_fiat_ind:= Induction for expr_pyro_to_fiat Sort Prop.
-Theorem expr_pyro_to_fiat_wf: 
-  forall (pt: term) A Gp
-  (Hpwf: pyro_expr_wf pt A Gp),
-  forall fe, Success fe = expr_pyro_to_fiat pt ->
-  exists ft Genv fenv Gstore fstore,
-  Success ft = ty_pyro_to_fiat A /\
-  Success Genv = env_pyro_to_fiat Gp /\
-  fenv_wf Gstore fstore /\
-  fenv_wf Genv fenv /\
-  type_of fstore fenv fe ft.
-Proof.
-  intros pt A Gp Hpwf. generalize A Gp.
-  induction pt using wf_judge_ind.
-
-  functional induction (expr_pyro_to_fiat pt); intros; inj_all; eauto.
-  - edestruct IHr; eauto; clear IHr.
-    edestruct IHr0; eauto; clear IHr0.
-    inj_all.
-    exists TBool
-    repeat eexists; eauto.
-
-
+End WithMap.
