translation/FiatToPyroSound.v
@@ -8,7 +8,6 @@ From Pyrosome Require Import Theory.Core Elab.Elab Tools.Matches Lang.SimpleVSub
 From Pyrosome Require Import Lang.FiatTest.
 Import Core.Notations.
 Import coqutil.Datatypes.Result Result.List Result.ResultMonadNotations.
-
 Require Import coqutil.Word.Interface coqutil.Word.Properties.
 
 Require Stdlib.derive.Derive.
@@ -20,32 +19,44 @@ Open Scope list.
 Require Import Stdlib.FSets.FMapInterface.
 Require Import Stdlib.ZArith.ZArith.
 
-Require coqutil.Map.SortedListString.
-Local Existing Instance SortedListString.map.
-Local Existing Instance SortedListString.ok.
-Local Existing Instance SortedListString.Build_parameters.
-
 Require Import Translator MapUtils Tactics.
-Import Stdlib.Sorting.Permutation.
-
-Opaque map.put map.get map.empty.
-
 Opaque fiat value_subst exp_subst.
 
+
+Section WithWord.
+  Context {width: Z} {word: word.word width}.
+  Context {word_ok: word.ok word}.
+
+Section WithMap.
+  Context {locals: forall T, map.map string T} 
+  {locals_ok: forall T, map.ok (locals T)}.
+
+Hint Unfold fenv_wf: core.
+Hint Resolve tenv_wf_ext: core.
+Hint Rewrite lookup_fmap: core. 
+Hint Resolve sorted_perm_eq: core.
+Hint Resolve fst_equal_equiv: core.
+Hint Rewrite lookup_fmap_none: core.
+Hint Constructors Forall2: core.
+Hint Resolve Forall2_map_left Forall2_map_right Forall2_split: core.
+
+Ltac fenv_reduce := inj_all;
+  repeat (match goal with
+  | [H: fenv_wf (?a::?b) ?c |-_] => apply fenv_wf_ext in H
+          end); map_simpl.
+
 Theorem type_lookup:
-  forall a x Gstore Genv {fstore:map.rep} {fenv:map.rep}
+  forall a x Gstore Genv {fstore:tenv} {fenv:tenv}
   (HFst: fenv_wf Gstore fstore)
   (HFenv: fenv_wf Genv fenv)
 (Hlookup: Success a = lookup_ind x Genv) {d},
   type_of fstore fenv (EVar x) (snd (nth a Genv d)).
 Proof.
-  induction a; intros; destruct Genv; fenv_reduce; econstructor; map_simpl.
+  induction a; intros; destruct Genv; fenv_reduce; do_both;
+  econstructor; map_simpl.
   rewrite <- lookup_fmap; eauto.
 Qed.
 Hint Resolve type_lookup: core.
-
-Require Import coqutil.Word.Naive.
-Local Existing Instance word32_ok.
 
 Theorem fiat_type_sound:
   forall Gstore Genv {fstore} {fenv} fe ft
@@ -55,8 +66,7 @@ Theorem fiat_type_sound:
   type_of fstore fenv fe ft.
 Proof.
   unfold get_fiat_type, fenv_wf.
-  intros.
-  inj_all.
+  intros. do_both.
   epose typechecker_sound; eauto.
   eapply proj1 in a1; eauto.
 Qed.
@@ -66,57 +76,16 @@ Hint Resolve fiat_type_sound: core.
 Ltac wf_term_ty := 
   lazymatch goal with
   | [H: Success ?a = ty_fiat_to_pyro ?ft ?Genv |- (wf_term _ _ ?a {{s #"ty"}})] => 
-    eapply ty_fiat_to_pyro_wf; try apply H; auto
+eapply ty_fiat_to_pyro_wf; try apply H; auto
  end.*)
 
-Theorem ty_fiat_to_pyro_wf:
-  forall ft
-  (Htwf: type_wf ft),
-  forall A
-  (Hty: Success A = ty_fiat_to_pyro ft),
-  wf_term (fiat++value_subst++exp_subst) [] A {{s#"ty"}}.
-
-Proof.
-  induction ft using type_IH; intros;
-  intros; inj_all; inversion Htwf; t''; eauto.
-  - match goal with [H:Success a = all_success (map ?f' l) |-_] => set (f:=f') in * end.
-
-    assert (map fst a = map fst l /\ StronglySorted (fun p p' => is_true (record_entry_leb p p')) a
-    ). {
-      generalize H2 case_match_eqn. clear.
-      generalize dependent a.
-      subst f.
-      induction l; intros; destruct a; invert_cons; apply conj; inj_all.
-      - eapply IHl; eauto.
-      - specialize (IHl a1).
-        constructor; inj_all.
-        assert (Hfst: Forall (fun n => is_true (s <=? n)) (map fst l)) by (rewrite Forall_map; eauto).
-        rewrite <- H in Hfst. rewrite Forall_map in Hfst; eauto.
-    } inj_all.
-
-    replace (record_sort a) with a in * by (eapply record_sort_iff_sorted; equality; eauto).
-
-    subst f.
-    repeat match goal with 
-           | [H: Success ?a = ?b|-_] => generalize H; clear H 
-           | [H: Forall ?a ?b|-_] => generalize H; clear H 
-           end.
-           clear. intros.
-   repeat match goal with
-           | [a: term|-_] => generalize dependent a 
-           | [a: list (string * _) |-_] => generalize dependent a 
-          end.
-    induction l; intros; destruct a; invert_cons; repeat (inj_all; t'').
-Qed.
-Hint Resolve ty_fiat_to_pyro_wf: core.
-
+(* Ltac to prove all_success of sorted records are typically sorted *)
 Ltac sort_success a0 :=
-    match goal with [H: Success a0 = all_success (map ?f ?tl'),
-    H': StronglySorted _ ?tl'
-    |-_] =>
+    lazymatch goal with [H: Success a0 = all_success (map ?f ?tl'),
+    H': StronglySorted _ ?tl'|-_] =>
     (assert (Hfst: map fst tl' = map fst a0) by (
       generalize H; clear; generalize dependent a0; induction tl'; intros; destruct a0; 
-        invert_cons; eauto);
+        invert_cons; do_both; eauto with permute);
     pose proof (fst_equal_equiv tl' a0); inj_all;
     assert (NoDup (map fst tl')) by eauto with permute;
 
@@ -127,6 +96,48 @@ Ltac sort_success a0 :=
     intros; rewrite record_sort_iff_sorted; repeat apply conj; try eapply fst_equal_equiv; eauto with permute);
     try erewrite <- Ha' in *; clear Ha'; eauto
     ) end.
+
+Theorem ty_fiat_to_pyro_wf:
+  forall ft
+  (Htwf: type_wf ft),
+  forall A
+  (Hty: Success A = ty_fiat_to_pyro ft),
+  wf_term (fiat++value_subst++exp_subst) [] A {{s#"ty"}}.
+
+Proof.
+  induction ft using type_IH; intros;
+  intros; do_both; inversion Htwf; t''.
+  - match goal with [H:Success a = all_success (map ?f' l) |-_] => set (f:=f') in * end.
+
+    assert (map fst a = map fst l /\ StronglySorted (fun p p' => is_true (record_entry_leb p p')) a
+). {
+      generalize H2 case_match_eqn. clear.
+      generalize dependent a.
+      subst f.
+      induction l; intros; destruct a; invert_cons; apply conj; invert_cons; do_both; eauto.
+      - constructor.
+      - eapply IHl; eauto.
+      - specialize (IHl a1); inj_all.
+        constructor; inj_all; eauto.
+        assert (Hfst: Forall (fun n => is_true (s <=? n)) (map fst l)) by (rewrite Forall_map; eauto).
+        rewrite <- H in Hfst. rewrite Forall_map in Hfst; eauto.
+    } inj_all.
+
+    subst f; sort_success a.
+
+    repeat match goal with 
+           | [H: Success ?a = ?b|-_] => generalize H; clear H 
+           | [H: Forall ?a ?b|-_] => generalize H; clear H 
+           end.
+           clear. intros.
+   repeat match goal with
+           | [a: term|-_] => generalize dependent a 
+           | [a: list (string * _) |-_] => generalize dependent a 
+          end.
+    induction l; intros; destruct a; invert_cons; do_both; t''.
+Qed.
+Hint Resolve ty_fiat_to_pyro_wf: core.
+
 
 Theorem ty_list_fiat_to_pyro_wf:
   forall l
@@ -146,13 +157,13 @@ Proof.
   assert (HDup': NoDup (map fst l')) by eauto with permute.
   clear HDup.
   eapply Permutation_Forall in Htwf; eauto.
-  inj_all.
+  do_both.
   match goal with [H: Success _ = all_success (map ?f' l)|-_] => set (f:=f') end.
   assert (Permutation (map f l) (map f l')) by eauto with permute.
   eapply all_success_permutation in case_match_eqn; eauto.
   clear dependent l.
 
-  inj_all.
+  do_both.
 
   unfold f in *.
   sort_success x.
@@ -163,7 +174,7 @@ Proof.
   generalize dependent lty.
   generalize dependent l'.
 
-  induction l'; intros; destruct x; invert_cons; try solve [t''; eauto].
+  induction l'; intros; destruct x; invert_cons; do_both; t''.
 Qed.
 Hint Resolve ty_list_fiat_to_pyro: core.
 
@@ -174,7 +185,7 @@ Theorem env_fiat_to_pyro_wf:
   wf_term (fiat++value_subst++exp_subst) [] Gp {{s#"env"}}.
 Proof.
   induction Genv as [|(n,t)];
-  intros; fenv_reduce; t''; eauto.
+  intros; fenv_reduce; do_both; t''.
 Qed.
 Hint Resolve env_fiat_to_pyro_wf: core.
 
@@ -185,7 +196,7 @@ Theorem env_fiat_to_pyro_contents_wf:
   wf_term (fiat++value_subst++exp_subst) [] A {{s#"ty"}} /\
   wf_term (fiat++value_subst++exp_subst) [] G {{s#"env"}}.
 Proof.
-  induction Genv as [|(n,t)]; intros; fenv_reduce.
+  induction Genv as [|(n,t)]; intros; fenv_reduce; do_both.
 Qed.
 
 Hint Resolve env_fiat_to_pyro_contents_wf type_of__type_wf: core.
@@ -202,11 +213,11 @@ Theorem get_ind_wkn_fiat_to_pyro_wf (n:nat):
   wf_term (fiat++value_subst++exp_subst) [] A {{s#"ty"}} /\
   forall {d}, Success A = ty_fiat_to_pyro (snd (nth (S n) Genv d))).
 Proof.
-  induction n; intros; destruct Genv; inj_all; fenv_reduce.
-  - repeat (try apply conj); t''; eauto.
-    intros. destruct Genv; inj_all. fenv_reduce. 
+  induction n; intros; destruct Genv; do_both; fenv_reduce; do_both.
+  - repeat apply conj; t''.
+    intros. destruct Genv; do_both. fenv_reduce; do_both; eauto.
   - edestruct IHn with (Genv:=Genv) as [HGp'' [HA Hind]]; eauto.
-    repeat (try apply conj); t''; eauto.
+    repeat apply conj; t''.
 Qed.
 Hint Resolve get_ind_wkn_fiat_to_pyro_wf: core.
 
@@ -220,16 +231,18 @@ Theorem get_ind_fiat_to_pyro_wf (n:nat):
 Proof.
   intros. 
   set (d:=("",TUnit)); specialize Hty with d.
-  destruct n; destruct Genv; fenv_reduce.
-  - t''; eauto.
-  - destruct n.
-    + destruct Genv; fenv_reduce; t''; eauto.
-    + specialize (get_ind_wkn_fiat_to_pyro_wf n H0) as H'.
-      destruct Genv; fenv_reduce. 
-      { destruct n; inj_all. }
-      edestruct H4; eauto; clear H4.
-      inj_all. specialize H8 with (s,t); rewrite <- H8 in Hty; inj_all.
-      t''; eauto.
+  destruct n; destruct Genv; fenv_reduce; do_both.
+  - t''.
+  - destruct n; do_both.
+    + destruct Genv; fenv_reduce; do_both. t''.
+    + specialize (get_ind_wkn_fiat_to_pyro_wf n) with (Genv:=Genv) (fenv:=x) as H';
+      do_both.
+      destruct Genv; fenv_reduce; do_both.
+      { destruct n; do_both. }
+      edestruct H'; eauto; clear H'; do_both.
+      edestruct H6; do_both.
+      specialize H9 with (s,t); rewrite <- H9 in Hty; do_both.
+      t''.
 Qed.
 Hint Resolve get_ind_fiat_to_pyro_wf: core.
 
@@ -242,6 +255,7 @@ Theorem record_ok:
   pt
   (He: Success pt = expr_fiat_to_pyro (ERecord l) Genv Gstore),
   let l' := record_sort l in
+  NoDup (map fst l') /\
   (map fst l') = (map fst tl') /\
   Forall2 (type_of fstore fenv) (map snd l') (map snd tl') /\
   StronglySorted (fun p p' => is_true (record_entry_leb p p')) tl' /\
@@ -252,17 +266,17 @@ Proof.
  specialize (StronglySorted_record_sort l) as Hsl. fold l' in Hsl.
  specialize (Permuted_record_sort l) as Hpl. fold l' in Hpl.
 
-  intros; invert_cons; inversion Hty; equality.
+  intros; invert_cons; inversion Hty; do_both.
 
   all: match goal with [H:Success ?a = all_success (map ?f' ?l)|-_] => set (f:=f') in * end.
   all: assert (Hpn: Permutation (map f l) (map f l')) by eauto with permute;
-    specialize (all_success_permutation Hpn) as Hs; inj_all; equality.
+    specialize (all_success_permutation Hpn) as Hs; inj_all; do_both.
 
     all: set (n := map fst l) in *; set (n' := map fst l') in *; inj_all;
     assert (Hpll': Permutation n n') by (unfold n, n'; eauto with permute);
     gather n; gather n'; assert (NoDup n') by eauto with permute.
 
-    all: unfold n', n, f in *; sort_success x; equality.
+    all: unfold n', n, f in *; sort_success x; do_both.
     clear dependent a1.
 
     assert (
@@ -274,7 +288,7 @@ Proof.
         apply Forall2_map_left with (f:=snd) in H2.
 
         assert (Hstrong: Forall2 (fun a b => type_of fstore fenv (snd a) (snd b) /\ fst a = fst b) l tl). {
-          apply Forall2_split; apply conj; eauto. rewrite Forall2_fst_eq; equality.
+          apply Forall2_split; apply conj; eauto. rewrite Forall2_fst_eq; do_both.
         }
         gather n.
         eapply Forall2_Permuted_StronglySorted in Hstrong; repeat apply conj; eauto; intros; inj_all;
@@ -288,9 +302,33 @@ Proof.
     repeat (apply conj; eauto).
     - apply Forall2_map_right with (f:=snd); apply Forall2_map_left with (f:=snd); eauto.
     - generalize case_match_eqn0; clear; generalize dependent x.
-      induction l'; intros; destruct x; invert_cons.
+      induction l'; intros; destruct x; invert_cons; do_both.
 Qed.
 Hint Resolve record_ok: core.
+
+Ltac inj_types_once := 
+  lazymatch goal with
+  | [H: Failure _ = lookup_ind _ ?G |-_] =>
+    eapply lookup_fmap_none with (Genv:=G) in H; eauto 2
+  | [Hty: Success ?ft = get_fiat_type ?fe ?Genv ?Gstore,
+      H: tenv_wf ?fenv,
+      H': Success ?fenv = fiat_env_to_map ?Genv |-_] =>
+      eapply fiat_type_sound in Hty; eauto 2
+  | [H: TList _ = TList _ |-_] => inversion H; clear H
+  | [H: TRecord _ = TRecord _ |-_] => inversion H; clear H
+  | [H: type_wf (TList _)|-_] => inversion H; clear H
+  | [Hty: type_of ?fstore ?fenv ?fe ?ft, Hty': type_of ?fstore ?fenv ?fe ?ft',
+      HGenv: tenv_wf ?fenv |-_] =>
+      assert (Heq: ft = ft') by eauto;
+      try assert (type_wf ft') by (eapply type_of__type_wf in Hty'; eauto);
+      clear Hty'
+  end.
+Ltac inj_types := repeat (try inj_types_once; inj_all; equality).
+
+Hint Resolve fiat_env_to_map_contains fiat_env_to_map_contents fenv_wf_ext: core.
+Hint Resolve fenv_wf_nil fenv_wf_cons: core.
+
+Set Ltac Profiling.
 
 Theorem type_of_unique:
   forall fe {fstore} {fenv} ft ft'
@@ -302,211 +340,45 @@ Theorem type_of_unique:
   pt
   (He: Success pt = expr_fiat_to_pyro fe Genv Gstore), ft = ft'.
 Proof.
-  induction fe using expr_IH; intros; inversion Hty; inversion Hty'; subst; try discriminate;
-  try solve [inj_all; equality;
-  invert_type_of; inj_all; equality; eauto].
-  - (* evar *)
-    equality.
-    assert (t1=t0) by eauto; subst.
-    assert (a0=t0) by eauto; subst.
-    eapply lookup_fmap_none with (fenv:=fenv) in case_match_eqn6; eauto.
-    eapply IHfe2 with (Genv := (x,t0)::Genv); eauto.
-    eapply fenv_wf_cons; eauto.
-    unfold fenv_wf in *; inj_all.
-    eapply type_of__type_wf in H3; eauto.
+  induction fe using expr_IH; intros; 
+  inversion Hty; inversion Hty'; simpl in *; subst; try discriminate;
+  try pose proof (record_ok Hty HFst HFenv He) as Hrec;
+  try pose proof (record_ok Hty' HFst HFenv He) as Hrec'; 
+  inversion HFst; inversion HFenv;
+  invert_type_of.
+  all: equality.
+  Show Ltac Profile.
+  all: inj_types.
   - (* records... *)
-    pose proof (record_ok Hty HFst HFenv He) as Hrec.
-    pose proof (record_ok Hty' HFst HFenv He) as Hrec'. 
-    inj_all.
-    specialize (StronglySorted_record_sort l) as Hsl.
-    specialize (Permuted_record_sort l) as Hpl.
-    f_equal.
     remember (record_sort l) as l' in *.
+    rewrite record_sort_iff_sorted in Heql'; inj_all; eauto with permute.
+    inj_all.
+    clear dependent a0.
+    sort_success a1.
+    rename a1 into a0.
+    f_equal.
     apply Permutation_forall with (l':=l') in H; eauto.
+    inj_all.
 
     clear dependent a0.
     clear dependent l.
+    do_both.
     clear dependent tl.
-    clear H10.
+    clear dependent tl0.
 
     generalize dependent tl'.
     generalize dependent tl'0.
-    induction l'; intros; destruct tl'0; destruct tl'; invert_cons.
-  - (* eaccess *)
-    specialize IHfe with (fstore:=fstore) (fenv:=fenv) (ft:=(TRecord tl)) (ft':=(TRecord tl0)) (Gstore:=Gstore) (Genv:=Genv); inj_all.
-    inversion IHfe; equality.
+    induction l'; intros; destruct tl'0; destruct tl'; invert_cons; 
+    f_equal; inj_types.
+  - (* ejoin *)
+    f_equal.
+    eapply IHfe4 with (Genv:=(y,a1)::(x,a0)::Genv); eauto.
+    eapply fenv_wf_cons; map_simpl; eauto; do_both.
+  - (* eproj *)
+    f_equal. eauto.
 Qed.
-    
-(*
-
-    match goal with [H:Success a0 = all_success (map ?f' l)|-_] => set (f:=f') in * end.
-    specialize (StronglySorted_record_sort l) as Hsl.
-    set (l':=(record_sort l)) in *.
-    set (a':=(record_sort a0)) in *.
-    assert (Hpl: Permutation (map f l) (map f l')) by eauto with permute.
-    specialize (all_success_permutation Hpl) as Hs; inj_all.
-
-    set (n := map fst l) in *; set (n' := map fst l') in *; inj_all.
-    assert (Hpll': Permutation n n') by (unfold n, n'; eauto with permute).
-
-
-      assert ((map fst x = map fst l') /\ StronglySorted (fun p p' => is_true (record_entry_leb p p')) x). {
-        clear Hpl. clear dependent a0. subst n n'; clear Hpll'.
-        generalize dependent x.
-        generalize dependent l'.
-        clear. 
-        unfold f, record_entry_leb in *.
-        induction l'; intros; invert_cons.
-        repeat (match goal with [a:?b*?c|-_]=>destruct a end).
-        apply conj; try f_equal; equality.
-        constructor; inj_all.
-        assert (Hfst: Forall (fun n => is_true (s <=? n)) (map fst l')) by (rewrite Forall_map; eauto).
-        rewrite <- H in Hfst. rewrite Forall_map in Hfst; eauto.
-      } inj_all.
-
-    assert (Hrec: x = a'). { 
-      fold n' in H7.
-      apply sorted_perm_eq; gather n'; gather n; unfold a'; eauto with permute. 
-    }
-
-    specialize (Permuted_record_sort l) as Hprl. fold l' in Hprl.
-
-    apply permutation_forall with (l':=l') in H; eauto.
-
-    (*
-    assert (
-    (map (fun p => (fst p, Success (fst (snd p)))) a0
-    = map (fun p => (fst p, expr_fiat_to_pyro (snd p) Genv Gstore)) l) /\
-    (map (fun p => (fst p, Success (snd (snd p)))) a0 
-    = map (fun p => (fst p, ty_fiat_to_pyro (snd p))) tl) /\
-    (map (fun p => (fst p, Success (snd (snd p)))) a0 
-    = map (fun p => (fst p, ty_fiat_to_pyro (snd p))) tl0)
-    ). {
-
-      induction l'; intros; destruct a0, tl, tl0; invert_cons.
-      repeat (match goal with [a:?b*?c|-_]=>destruct a end); inj_all.
-      assert (a2=t1) by eauto; 
-      assert (a2=t2) by eauto; equality.
-      edestruct IHl with (tl:=tl) (tl0:=tl0); inj_all; eauto; equality.
-      repeat (try apply conj; try f_equal); equality.
-    } inj_all.
-    (*
-    apply permutation_forall with (l':=l') in H; eauto.
-
-    subst l'. remember (record_sort l) as l'.
-    gather x; gather l'; gather tl'; gather tl0'.
-    clear dependent l.
-    clear dependent a0. 
-    clear dependent tl. 
-    clear dependent tl0. 
-    rename x into a0'.
-    
-     *)
-     *)
-    
-    assert (Hpy: Forall 
-      (fun p => exists pt, Success pt = expr_fiat_to_pyro (snd p) Genv Gstore)  
-      l'). { 
-        subst n n'; clear Hpll'.
-        gather x. clear dependent a0.
-        generalize dependent t.
-        generalize dependent t0.
-        generalize dependent x.
-        clear Hpl Hprl.
-        induction l'; intros; inj_all.
-        repeat (match goal with [a:?b*?c|-_]=>destruct a end).
-        unfold f in *.
-        eapply Forall_cons; invert_cons; eauto.
-      }
-
-    assert (
-      Forall2 (fun a b => type_of fstore fenv (snd a) (snd b)) l' tl' /\
-      Forall2 (fun a b => type_of fstore fenv (snd a) (snd b)) l' tl'0 /\
-      n' = map fst tl' /\
-      n' = map fst tl'0
-    ). {
-      unfold n'.
-        apply Forall2_map_right with (f:=snd) in H2, H9;
-        apply Forall2_map_left with (f:=snd) in H2, H9.
-
-        assert (Hstrong: Forall2 (fun a b => type_of fstore fenv (snd a) (snd b) /\ fst a = fst b) l tl). {
-          apply Forall2_split; apply conj; eauto. rewrite Forall2_fst_eq; equality.
-        }
-        assert (Hstrong0: Forall2 (fun a b => type_of fstore fenv (snd a) (snd b) /\ fst a = fst b) l tl0). {
-          apply Forall2_split; apply conj; eauto. rewrite Forall2_fst_eq; equality.
-        }
-        gather n.
-        eapply Forall2_Permuted_StronglySorted in Hstrong, Hstrong0; repeat apply conj; eauto; intros; inj_all;
-        try solve [eapply Forall2_impl; eauto; intros; inj_all];
-        apply Forall2_fst_eq;
-        apply Forall2_impl with (R2:=(fun a b => fst a = fst b)) in Hstrong, Hstrong0; intros; inj_all.
-      } inj_all.
-      subst l'. 
-      remember (record_sort l) as l' in *.
-      subst a'.
-      remember (record_sort a0) as a' in *.
-    subst n'.
-    remember (map fst l') as n' in *.
-    clear dependent a0.
-    clear dependent l.
-    clear dependent tl.
-    clear dependent tl0.
-    inj_all.
-
-    assert (tl'=tl'0). {
-      generalize dependent t;
-      generalize dependent t0;
-      generalize dependent tl';
-      generalize dependent tl'0;
-      generalize dependent a'.
-        induction l'; intros; destruct tl'; destruct tl'0; invert_cons.
-    } inj_all.
-
-    (*
-        apply Forall2_map_right with (f:=snd);
-        apply Forall2_map_left with (f:=snd);
-        apply Forall2_map_right with (f:=snd) in H2;
-        apply Forall2_map_left with (f:=snd) in H2.
-
-        set (n := map fst l) in *; gather n; inj_all.
-        intros; inj_all.
-        Compute Forall2_Permuted_StronglySorted.
-    }
-
-      apply permutation_forall with (l':=l) in Hpy; eauto with permute.
-
-      assert (tl = tl0). {
-        clear dependent x.
-        clear case_match_eqn0 Hty Hty'.
-        generalize dependent l.
-        generalize HFst HFenv Heq.
-        clear.
-        intros.
-        generalize dependent tl.
-        generalize dependent tl0.
-        generalize dependent l.
-        induction l; intros; inj_all;
-        destruct tl; try solve [inversion H2; eauto];
-        destruct tl0; try solve [inversion H9; eauto].
-        repeat (match goal with [a:?b*?c|-_]=>destruct a end).
-        subst l' n; invert_cons.
-        repeat (f_equal; inj_all; eauto).
-        eapply IHl; eauto with permute.
-      } inj_all.
-      assert (tl'=tl'0); inj_all.
-      apply sorted_perm_eq; eauto with permute.
-     *)
-Qed.
- *)
 
 Hint Resolve type_of_unique: core.
-Ltac inj_types := try repeat (
-  try match goal with
-  | [Hty: Success ?ft = get_fiat_type ?fe ?Genv ?Gstore, Hty': type_of ?fstore ?fenv ?fe ?ft' |-_] =>
-      assert (Hfteq: ft=ft') by eauto;
-      assert (type_wf ft') by (apply type_of__type_wf in Hty'; eauto);
-      clear Hty'
-  end; equality); inj_all.
 
 Definition fiat_rules := fiat ++ value_subst ++ exp_subst.
 
@@ -514,7 +386,7 @@ Definition pyro_expr_wf (pexpr: term) (pty: term) (penv: term) :=
   wf_term fiat_rules [] pexpr (scon "val" [pty;penv]).
 
 Theorem expr_fiat_to_pyro_wf:
-  forall fe Gstore Genv (fstore:map.rep) (fenv:map.rep) ft
+  forall fe Gstore Genv (fstore:tenv) (fenv:tenv) ft
   (HFst: fenv_wf Gstore fstore)
   (HFenv: fenv_wf Genv fenv)
   (Hty: type_of fstore fenv fe ft),
@@ -525,152 +397,153 @@ Theorem expr_fiat_to_pyro_wf:
   pyro_expr_wf pt A Gp.
 Proof.
   unfold pyro_expr_wf in *;
-  induction fe using expr_IH; simpl; inj_all; intros;
-  inversion HFenv;
-  inversion HFst;
-  inversion Hty; clear Hty; invert_type_of; inj_types; try solve [t''; eauto].
-  (*symmetry in case_match_eqn; 
-  pose proof env_fiat_to_pyro_wf Genv HGenv HFenv case_match_eqn as HGenv_wf.*)
-  - eapply get_ind_fiat_to_pyro_wf; eauto; intros.
+  induction fe using expr_IH; intros;
+  inversion Hty; simpl in *; subst; try discriminate;
+  try pose proof (record_ok Hty HFst HFenv He) as Hrec;
+  inversion HFenv; inversion HFst;
+  invert_type_of.
+
+  (* now this part takes about fifty years *)
+  all: inj_types. 
+  all: try solve [t''].
+
+  Show Ltac Profile.
+  Unset Ltac Profiling.
+  - (* evar, of course *)
+    eapply get_ind_fiat_to_pyro_wf; eauto; intros.
     assert (Hty': type_of fstore fenv (EVar x) (snd (nth a0 Genv d))). {
       eapply type_lookup; eauto.
-    }
-    inversion Hty'; equality.
+    } inversion Hty'; do_both.
+
   - (* cons *)
-    assert (Success (con "list" [a0]) = ty_fiat_to_pyro (TList t1)) by inj_all.
-    t''; eauto.
+    assert (Success (con "list" [a]) = ty_fiat_to_pyro (TList a3)) by inj_all.
+    t''.
+
   - (* let *)
-    eapply lookup_fmap_none with (fenv:=fenv) in case_match_eqn6; eauto.
     specialize (fenv_wf_cons HFenv) as Hewf.
-    edestruct Hewf with (x:=x) (a:=t1); eauto.
+    edestruct Hewf with (x:=x); clear Hewf; eauto 2.
     inj_types.
-
     assert (pyro_expr_wf a3 A (con "ext" [a4;a])). {
-      eapply IHfe2 with (Gstore:=Gstore) (Genv:=(x,t1)::Genv); eauto.
-      inj_all.
+      eapply IHfe2 with (Gstore:=Gstore) (Genv:=(x,a0)::Genv); eauto.
+      do_both.
     }
+    t''.
 
-    t''; eauto.
   - (* record my beloathed... *)
-    assert (Hty: type_of fstore fenv (ERecord l) (TRecord tl')) by (econstructor; eauto).
-    assert (He: Success t = expr_fiat_to_pyro (ERecord l) Genv Gstore) by inj_all.
-    pose proof (record_ok Hty HFst HFenv He) as Hrec.
-    inj_all.
-    specialize (StronglySorted_record_sort l) as Hsl.
     specialize (Permuted_record_sort l) as Hpl.
-    f_equal.
     remember (record_sort l) as l' in *.
-    rewrite record_sort_iff_sorted in Heql'; equality.
+    rewrite record_sort_iff_sorted in Heql'; eauto with permute.
+    inj_all.
 
-    clear dependent a4.
+    match goal with [H: Success ?x = all_success (map _ l) |-_] => clear dependent x end.
     apply Permutation_forall with (l':=l') in H; eauto.
 
    remember (map fst l') as n' in *.
    assert (NoDup (map fst tl')) by eauto with permute.
     assert (NoDup n') by (gather n'; eauto with permute).
-    sort_success a0. equality.
-    sort_success a. equality.
+    sort_success a1. do_both.
+
+    rename Hfst into Hfst'.
+    sort_success a0. do_both.
+    rename Hfst into Hfst''.
+    
+    inj_types.
 
     clear dependent l.
     clear dependent tl.
+    clear t2.
 
+    rename t1 into t3.
+    rename t0 into t2.
+    rename a into a3.
 
-    (*
-    generalize dependent tl'.
-    generalize dependent a1.
-    generalize dependent t1.
-    generalize dependent t2.
-    
-
-    assert (StronglySorted (fun p p' => is_true (Value.record_entry_leb p p')) l') by eauto using StronglySorted_record_sort.
-    (*
-    assert (StronglySorted (fun p p' => is_true (Value.record_entry_leb p p')) tl). {
-      generalize l H5 H8 H4; clear.
-      induction tl; intros; destruct l; invert_cons; econstructor; eauto.
-      destruct p, a; unfold Value.record_entry_leb in *; inj_all.
-      assert (Forall (fun p => is_true (s0<=? p)) (map fst l)). {
-        rewrite Forall_map; eauto.
-      }
-      rewrite H3 in H.
-      rewrite Forall_map in H; eauto.
-   }
-      assert (NoDup (map fst tl) /\ NoDup (map fst tl')) by
-      (apply conj;
-        eauto using Permutation.Permutation_NoDup, Permutation.Permutation_map).
-      inj_all.
-    assert (tl=tl') by eauto using sorted_perm_eq.
-   *)
-    invert_cons.
-     *)
-    rename a1 into a2.
-
-    assert ((pyro_expr_wf t1 (con "Trecord" [a2]) a3 /\ 
+    assert ((pyro_expr_wf t3 (con "Trecord" [a2]) a3 /\ 
     Success (con "Trecord" [a2]) = ty_fiat_to_pyro (TRecord tl')) /\
     wf_term (fiat++value_subst++exp_subst) [] a2 (scon "list_ty" []) /\
     t2 = a2
     ). {
-      unfold pyro_expr_wf in *. equality.
-      all: clear Hfst; sort_success a1.
-      all: clear Heq; equality.
-      inj_all.
+      unfold pyro_expr_wf in *. do_both.
+      all: sort_success a; inj_all; do_both.
 
-      generalize dependent tl'.
-      generalize dependent a.
-      generalize dependent a0.
-      generalize dependent a1.
-      generalize dependent a3.
-      generalize dependent t0.
-      generalize dependent t1.
-      generalize dependent t2.
-      generalize HFst HFenv.
-      generalize dependent l'.
-      clear.
+      repeat match goal with 
+             | [a: term |-_] => generalize dependent a
+             | [l: list _ |-_] => generalize dependent l 
+             end.
 
-      induction l'; intros; destruct tl'; destruct a; destruct a1; invert_cons. 
-      - repeat (apply conj); t''; eauto.
+      induction l'; intros; destruct tl'; destruct a; destruct a0; invert_cons. 
+      - repeat apply conj; t''.
       - inversion HFst. inversion HFenv.
         inj_types.
-      edestruct IHl'; eauto; clear IHl'; inj_all; equality.
-      repeat (apply conj; t''; eauto).
+      edestruct IHl'; eauto; clear IHl'; inj_all; do_both.
+      repeat apply conj; t''.
     } inj_all.
 
-  - inversion Hfteq; inj_all.
-    inversion H3; clear H3; inj_all. (* type wf *)
+  - (* EAccess *)
+    match goal with [H: type_wf (TRecord _)|-_] => inversion H; clear H end.
+    inj_all.
+
     assert (Hpwf: pyro_expr_wf a0 (con "Trecord" [a1]) a). {
       eapply IHfe with (fenv:=fenv) (fstore:=fstore); eauto.
-      eauto.
       unfold ty_list_fiat_to_pyro, ty_fiat_to_pyro in *.
-      generalize case_match_eqn2; clear. generalize dependent a1.
-      induction tl; intros; destruct a1; invert_cons.
-    } clear dependent fe.
+      inj_all.
+    } 
     unfold pyro_expr_wf in *.
+    clear dependent fe.
 
     assert (Hlty: forall tl, StronglySorted (fun p p' => is_true (record_entry_leb p p')) tl
-  -> Forall type_wf (map snd tl) -> NoDup (map fst tl) -> 
-    forall a1, Success a1 = ty_list_fiat_to_pyro tl ->
-    wf_term fiat_rules [] a1 (scon "list_ty" [])
+    -> Forall type_wf (map snd tl) -> NoDup (map fst tl) -> 
+      forall a1, Success a1 = ty_list_fiat_to_pyro tl ->
+      wf_term fiat_rules [] a1 (scon "list_ty" [])
     ). {
-      intros.
-      eapply ty_list_fiat_to_pyro_wf; eauto.
+      intros; eapply ty_list_fiat_to_pyro_wf; eauto.
     }
     unfold ty_list_fiat_to_pyro, make_list_ty in *.
     inj_all.
-    sort_success a3; equality.
+    sort_success a3; do_both.
 
     repeat (match goal with 
             | [a:term|-_] => generalize dependent a 
             end).
     generalize dependent s.
     generalize dependent a3.
-    generalize dependent tl.
+    generalize dependent l.
     generalize dependent ft.
     generalize dependent a2.
 
-    induction a2; intros; destruct tl; simpl in *; try discriminate;
+    induction a2; intros; destruct l; simpl in *; try discriminate;
     invert_cons; try contradiction.
      * sort_success a4; inj_types.
-       t''; eauto. eapply Hlty; inj_all; eauto; sort_success a1.
+       t''. eapply Hlty; inj_all; eauto; sort_success a1.
      * sort_success a5; inj_types.
-       eapply IHa2 with (ft:=ft) (tl:=tl) (s:=s); eauto.
-       t''; eauto. eapply Hlty; inj_all; eauto; sort_success a2.
+       eapply IHa2 with (ft:=ft) (l:=l) (s:=s); eauto.
+       t''. eapply Hlty; inj_all; eauto; sort_success a1.
+
+  - (* EFilter *)
+    t''; cbn.
+     * eapply IHfe2 with (Genv:=(x,a1)::Genv) (Gstore:=Gstore); inj_all; eauto.
+     * eapply IHfe1 with (Genv:=Genv) (Gstore:=Gstore); eauto; inj_all.
+  - (* EJoin *)
+    specialize (fenv_wf_cons HFenv) with (x:=x) (a:=a1) as HFenv'; inj_all.
+    specialize (fenv_wf_cons HFenv') with (x:=y) (a:=a2) as HFenv''; map_simpl.
+    inversion HFenv'; inversion HFenv''.
+    inj_types.
+
+    eapply IHfe4 in case_match_eqn13; eauto 2; inj_all.
+    eapply IHfe3 in case_match_eqn12; eauto 2; inj_all.
+    eapply IHfe2 in case_match_eqn11; eauto 2; inj_all.
+    eapply IHfe1 in case_match_eqn10; eauto 2; inj_all.
+
+    t''.
+
+  - (* EProj *)
+    specialize (fenv_wf_cons HFenv) with (x:=x) (a:=a2) as HFenv'; inj_all.
+    inversion HFenv'.
+    inj_types.
+
+    eapply IHfe2 in case_match_eqn7; eauto 2; inj_all.
+    eapply IHfe1 in case_match_eqn1; eauto 2; inj_all.
+
+    t''.
 Qed.
+End WithMap.
+End WithWord.
