translation/Tactics.v
@@ -10,6 +10,7 @@ Import Core.Notations.
 Import coqutil.Datatypes.Result Result.List Result.ResultMonadNotations.
 
 Require Import coqutil.Word.Interface coqutil.Word.Properties.
+Export Stdlib.Sorting.Permutation.
 
 Require Stdlib.derive.Derive.
 Require Import Datatypes.String Lists.List.
@@ -20,55 +21,92 @@ Open Scope list.
 Require Import Stdlib.FSets.FMapInterface.
 Require Import Stdlib.ZArith.ZArith.
 
-Ltac inj_all := repeat (try case_match;
+Ltac t'' := repeat (
   match goal with
-  | [H: (Success ?a) = (Success ?b) |- _] => injection H as H
-  | [H: (Failure ?a) = (Failure ?b) |- _] => injection H as H
-  | [H: (Some ?a) = (Some ?b) |- _] => injection H as H
+  | [|-Model.wf_term _ _ _] => t'
+  | [|-wf_term _ _ _ _] => eapply wf_term_by'
+  | [|-wf_args _ _ _] => econstructor
+  | [|-_] => unshelve (repeat t); simpl
+  end); eauto 2.
+
+Ltac inj_all_once:= (
+  simpl in *; subst; try discriminate; try contradiction; auto;
+  try lazymatch goal with
   | [H: exists a, ?b |- _] => destruct H
   | [H: ?a /\ ?b |- _] => destruct H
-  | [H: ?a =? ?b = true |-_] => try rewrite String.eqb_eq in H
-  | [H: ?a =? ?b = false |-_] => try rewrite String.eqb_neq in H
   | [H: ?a = ?a |-_] => clear H
+  | [H: ?a = ?b, H': ?a = ?b |-_] => clear H'
   | [H: forall a, Success a = Success ?b -> ?P |-_] => 
-      assert (Heq: Success b = Success b) by auto; 
-      specialize (H b Heq); clear Heq
+      try (assert (Heq: Success b = Success b) by auto; 
+      specialize (H b Heq); clear Heq)
   | [H: forall a a', Success (a, a') = Success (?c, ?c') -> ?P |-_] => 
-      assert (Heq: Success (c,c') = Success (c,c')) by auto; 
-      specialize (H c c' Heq); clear Heq
+      try (assert (Heq: Success (c,c') = Success (c,c')) by auto; 
+      specialize (H c c' Heq); clear Heq)
   | [H: forall a, Success a = ?b -> ?P, H': Success ?c = ?b |-_] => 
       specialize (H c H')
-  | [|- _] => discriminate
-  | [H: ?b = Success ?a |- _] => symmetry in H
-  | [H: ?b = Failure ?a |- _] => symmetry in H
-  | [H: Forall ?p (?a::?b) |- _] => inversion H; clear H
-  | [H: Forall2 ?p (?a::?b) (?c::?d) |- _] => inversion H; clear H
-  | [H: (?a::?b)=(?c::?d) |-_] => inversion H; clear H
-  | [H: (?a,?b)=(?c,?d) |-_] => inversion H; clear H
-  | [H: ?a, H': ~?a |-_] => contradiction
-  | [H: ?a->?b |-_] => assert (Hnew: a) by auto; specialize (H Hnew); clear Hnew
   | [a: ?b * ?c |-_] => destruct a 
-  | [|- _] => solve [repeat (f_equal); eauto]
-  | [|- (?a,?b)=(?c,?d)] => assert (a=c) by eauto; f_equal; eauto
-  | [|- (?a,?b)=(?c,?d)] => assert (b=d) by eauto; f_equal; eauto
-  | [|- ?a::?b = ?c::?d] => assert (a=c) by eauto; f_equal; eauto
-  | [|- ?a::?b = ?c::?d] => assert (b=d) by eauto; f_equal; eauto
-  | [H: ?P ?b |- ?P ?a] => solve [assert (Heq: a=b) by eauto; rewrite Heq; eauto]
+  | [H: (?a,?b)=(?c,?d) |-_] => inversion H; clear H
   | [H: NoDup ?x, H': NoDup ?x|-_] => clear H'
   | [H: StronglySorted ?x ?y, H': StronglySorted ?x ?y|-_] => clear H'
-  | [|- _] => idtac
-  end; simpl in *; subst; auto).
+  | [H: type_wf ?x, H': type_wf ?x|-_] => clear H'
+  | [H: type_of ?x ?y ?z ?w, H': type_of ?x ?y ?z ?w|-_] => clear H'
+  | [H: ?a =? ?b = true |-_] => rewrite String.eqb_eq in H
+  | [H: ?a =? ?b = false |-_] => rewrite String.eqb_neq in H
+  | [H: ?a->?b, H': ?a |-_] => specialize (H H')
+  | [H: (?a = ?a)->?b |-_] => assert (H':a=a) by eauto; specialize (H H'); clear H'
+  | [H: (Success ?a) = (Success ?b) |- _] => injection H as H; subst
+  | [H: (Failure ?a) = (Failure ?b) |- _] => injection H as H; subst
+  | [H: (Some ?a) = (Some ?b) |- _] => injection H as H; subst
+  | [H: ?b = Success ?a |- _] => symmetry in H
+  | [H: ?b = Failure ?a |- _] => symmetry in H
+  | [H: ?P ?b |- ?P ?a] => try solve [assert (Heq: a=b) by eauto; rewrite Heq; eauto]
+  end).
 
-Ltac equality := repeat (match goal with
+Ltac inj_all := repeat (repeat inj_all_once; try case_match); auto.
+
+Ltac equality_once := try (lazymatch goal with
+  | [H: Success ?a = ?b, H': Success ?c = ?b |-_] => assert (Heq: Success a = Success c) by (rewrite H; rewrite H'; auto); injection Heq as Heq; subst
+  | [H: Success ?a = ?b, H': Failure ?c = ?b |-_] => assert (Success a = Failure c) by (rewrite H; rewrite H'; auto); discriminate
   | [H: ?a = ?b, H': ?a = ?c |-_] => match a with None => idtac | _ => rewrite H in H'; subst end
-  | [H: ?a = ?b, H': ?b = ?c |-_] => rewrite H' in H; subst
-  | [H: ?a = ?b, H': ?c = ?b |-_] => assert (Heq: a=c) by (rewrite H; auto); inj_all
-  | [H: Success ?a = ?b, H': Success ?c = ?b |-_] => assert (Heq': Success a = Success c) by (rewrite H; rewrite H'; auto); injection Heq' as Heq'; subst
-  | [H: ?a = ?c, H': ?b = ?c |- ?a = ?b] => rewrite H; rewrite H'; auto
-  | [H: ?P ?a, H': ?a = ?b |- ?P ?b ] => rewrite H'; auto
-  | [H: ?P ?a, H': ?b = ?a |- ?P ?b ] => rewrite H'; auto
-  | [|-_] => idtac
-                 end; subst; try discriminate); inj_all.
+      (*
+         | [H: ?a = ?b, H': ?b = ?c |-_] => rewrite H' in H; subst*)
+  | [H: ?a = ?c, H': ?b = ?c |- ?a = ?b] => solve [rewrite H; rewrite H'; auto]
+  end; inj_all_once); try match goal with 
+  | [H: ?P ?a |- ?P ?b ] => try solve [assert (H':b=a) by eauto; rewrite H'; auto] 
+  | [|- (?a,?b)=(?c,?d)] => try (assert (a=c) by eauto; f_equal; auto); 
+                            try (assert (b=d) by eauto; f_equal; auto)
+  | [|- ?a::?b = ?c::?d] => try (assert (a=c) by eauto; f_equal; auto); 
+                            try (assert (b=d) by eauto; f_equal; auto)
+  | [|- _] => try solve [repeat (f_equal); auto]
+  end.
+
+Ltac equality := repeat (inj_all_once; equality_once); auto.
+Ltac do_both := repeat (equality; inj_all); eauto.
+
+Ltac invert_cons := repeat (
+  try match goal with
+  | [H: NoDup (?b::?c) |-_] => inversion H; clear H
+  | [H: StronglySorted ?a (?b::?c) |-_] => inversion H; clear H
+  | [H: Permutation [] (?a::?b) |-_] => eapply Permutation_nil in H
+  | [H: Permutation (?a::?b) [] |-_] => eapply Permutation_sym in H; eapply Permutation_nil in H
+  | [H: Permutation ?a ?a |-_] => clear H
+  | [H: Forall2 ?p [] (?a::?b) |-_] => inversion H
+  | [H: Forall2 ?p (?a::?b) [] |-_] => inversion H
+  | [H: Forall ?p (?a::?b) |-_] => inversion H; clear H
+  | [H: Forall2 ?p (?a::?b) (?c::?d) |- _] => inversion H; clear H
+  | [H: (?a::?b)=(?c::?d) |-_] => inversion H; clear H
+  end; inj_all).
+
+Global Hint Constructors Permutation: permute.
+Global Hint Resolve Permuted_record_sort
+  Permutation_map
+  Permutation_in
+  Permutation_NoDup
+  Permutation_refl
+  Permutation_sym
+  Permutation.Permutation_cons_inv 
+  Permutation_trans: permute.
+Global Hint Resolve in_eq in_map: core.
 
 Ltac invert_type_of := repeat (
   match goal with
@@ -79,7 +117,13 @@ Ltac invert_type_of := repeat (
   end; subst; try discriminate).
 
 Search "get".
-Ltac map_simpl := repeat (match goal with
+Ltac map_simpl := repeat (
+  try (erewrite map.get_put_same in * by eauto; inj_all);
+  try (erewrite map.get_put_diff in * by eauto; inj_all);
+  try (erewrite map.get_empty in * by eauto; inj_all)
+  ).
+  (*
+  match goal with
   | [H: map.get (map.put ?m ?k ?v) ?k = _ |-_] => erewrite map.get_put_same in H
   | [H: _ = map.get (map.put ?m ?k ?v) ?k |-_] => erewrite map.get_put_same in H
   | [|- _ = map.get (map.put ?m ?k ?v) ?k] => erewrite map.get_put_same
@@ -93,4 +137,10 @@ Ltac map_simpl := repeat (match goal with
   | [H: _ = map.get map.empty ?k |-_] => erewrite map.get_empty in H
   | [|- map.get map.empty ?k = _] => erewrite map.get_empty
   | [|- _ = map.get map.empty ?k] => erewrite map.get_empty
-end; auto); auto.
+   *)
+
+Ltac gather n :=
+  repeat match goal with
+         | [H: n = ?m|-_] => rewrite <- H in *
+         | [H: ?m = n|-_] => rewrite H in *
+         end.
