translation/README.md
@@ -1,0 +1,56 @@
+# fiat-pyrosome translator
+
+## structure + roadmap
+
+(as of 02 june 2026)
+
+run `make -j16` to build. `pyrosome` and `fiat2` build fine let's keep it that way
+
+- `Translator.v` (contains actual translation functions)
+  - [x] fiat to pyro is good and has some interesting stuff
+  - [ ] pyro to fiat is more rudimentary atm
+    - [ ] need variable naming (the sorting order is wrong. annoying)
+- `FiatToPyroSound.v` (proofs)
+  - [x] type safety proof (works well! for now)
+    - [x] tactics run in reasonable time 
+- `PyroToFiatSound.v` (proofs)
+  - [ ] type safety proof
+    - [ ] **blocker: value sort equivalence: figure out subst / contexts**
+    - [ ] sorting admits (see translator.v)
+  - [ ] some cleanup? (things are named stupidly and unreferenceable)
+  - i could probably write a tactic for rule checks (currently it's `repeat [destruct H; equality]`)
+
+## things to note before i forget
+
+### how to induct on pyrosome terms
+
+`BoolLang.v` (for reference) is [here](https://github.com/DIJamner/pyrosome/blob/623eb535d87bbb6fb9aabb4a656ccbfa4d0bd3fd/WIP/BoolLang.v)
+
+notes from meeting: 
+
+```
+judgement induction should...
+
+   one level of induction -- there's a lemma for that...
+   eq_sort causes issues...
+   the t being scon ty directly might be bad for induction in rocq / you don't want to lose the generality
+   the ty thing: induction rather than conclusion
+   and rocq equality rather than eq_sort
+
+   lemma: sort equality on ty, list_ty has to...
+   ref boollang.v
+
+   list_ty and ty: manually write a lemma for cases
+```
+
+dealing with `wf_args`: repeated destruct is fine
+
+### tactics
+
+- custom tactics are in `Tactics.v`
+- `eauto` takes infinite time, be careful. 90% of things being slow is that
+  - use auto or limit scope where possible
+  - `eauto 2` works well
+- tactic profiling: `Set Ltac Profiling` to start profiling and `Show Ltac Profile` to well show profile
+  - but this will **timeout with pyrosome terms** (`{{e {x} ...}}`) so make sure you disable it
+- `cbn` is useful `intuition` is useful
